Several minor improvements.

TopologicalSorting.dfy
@@ -1,33 +1,33 @@
 /*
- * Proof of correctness of the classic topological sorting algorithm (Kahn's algorithm), simplified, in Dafny.
- * Difficulty: High.
- * FEUP, MIEIC, MFES, 2020/21.
- * TODO: Improve the definition of simple path.
+ * Proof of correctness of the classic topological sorting algorithm (Kahn's algorithm),
+ * simplified, in Dafny.
+ * João Pascoal Faria (jpf@fe.up.pt), FEUP, January, 2022.
 */
 
 // Defines a directed graph with vertices of any type T as a pair (V, E), where V is the 
 // vertex-set and E is the edge-set. Each directed edge is represented by a pair of vertices. 
 datatype Graph<T> = Graph(V: set<T>, E: set<(T,T)>) 
 
-// Checks if G defines a valid graph.           
+// Checks if G defines a valid graph (checks that E is a subset of V*V).           
 predicate validGraph<T>(G: Graph<T>) {
   forall e :: e in G.E ==> e.0 in G.V && e.1 in G.V
 }
 
 // Checks if a graph is acyclic.
 predicate acyclic<T>(G: Graph<T>) {
-  ! exists v :: v in G.V && existsSimplePath(G, v, v) 
+   ! exists v :: v in G.V && existsSimplePath(G, v, v) 
 }
 
 // Check if there is a non-empty simple path from vertex u to vertex v in graph G.
-// (Currently, 'simple' means without repeated edges, but should be without repeated vertices).
+// (Currently, 'simple' means without repeated edges, but could be without repeated vertices).
 predicate existsSimplePath<T>(G: Graph<T>, u: T, v: T)
   decreases G.E
 {
   (u, v) in G.E || exists e :: e in G.E && e.0 == u && existsSimplePath(Graph(G.V, G.E-{e}), e.1, v) 
 }
 
-// Removes a vertex v and incident edges from a graph G.
+
+// Removes a vertex v and its incident edges from a graph G.
 function method removeVertex<T>(v: T, G: Graph<T>) : Graph<T> {
     Graph(G.V - {v}, set e | e in G.E && e.0 != v && e.1 != v)
 }  
@@ -41,6 +41,12 @@ predicate isTopSorting<T>(s: seq<T>, G: Graph<T>)
   && forall i, j:: 0 <= i <= j < |s| ==> (s[j], s[i]) !in G.E  
 }
 
+// Checks if a vertex v in a graph G has incoming edges.
+predicate method hasIncomingEdges<T>(G: Graph<T>, v: T) 
+ requires v in G.V
+{
+  exists u :: u in G.V && (u, v) in G.E
+}
 
 // Topological sorting of the vertices of an acyclic directed graph.
 // Returns a sequence (linear ordering) of the vertices in topological ordering.
@@ -49,53 +55,50 @@ method topsort<T>(G: Graph<T>) returns (s: seq<T>)
   ensures isTopSorting(s, G)
 {
   s := [];
-  var G' := G; // remaining graph
-  while G'.V != {} 
-    // relation between s and G' (basically, G' = G - s)
-    invariant G' == Graph(set v | v in G.V && v !in s, set e | e in G.E && e.0 !in s && e.1 !in s)
-    // remaining graph keeps same properties of initial one
-    invariant validGraph(G) && acyclic(G')
-    // s is a topological sort of G - G' 
-    invariant multiset(s) == multiset(G.V - G'.V) 
+  var R := G; // remaining graph
+  while R.V != {} 
+    // relation between s and R (basically, R = G - s)
+    invariant R == Graph(set v | v in G.V && v !in s, set e | e in G.E && e.0 !in s && e.1 !in s)
+    // s is a topological sorting of G - R 
+    invariant multiset(s) == multiset(G.V - R.V) 
     invariant forall i, j:: 0 <= i <= j < |s| ==> (s[j], s[i]) !in G.E  
-    // s is not any subset: there are no edges from vertices in G' to vertices in s 
-    invariant forall i:: 0 <= i < |s| ==> forall v :: v in G'.V ==> (v, s[i]) !in G.E  
-    decreases G'.V
+    // there are no edges from vertices in R to vertices in s 
+    invariant forall i:: 0 <= i < |s| ==> forall v :: v in R.V ==> (v, s[i]) !in G.E  
+    decreases R.V
   {
-    // recalls property that a vertex without incoming edges must exist in a non-empty acyclic graph
-    lemmaAcyclic(G');
+    // recall property: a subgraph of an ayclic graph is also acyclic 
+    lemmaAcyclicSubgraph(R, G);
+
+    // recall property: a vertex without incoming edges must exist in
+    // a non-empty acyclic graph
+    lemmaAcyclicIndegrees(R);
 
     // pick a vertex without incoming edges
-    var v :| v in G'.V && !exists u :: u in G'.V && (u, v) in G'.E; 
+    var v :| v in R.V && !hasIncomingEdges(R, v); 
 
     // append to the result
     s := s + [v];
      
-    // recalls property that removing a vertex from an ayclic graph produces an acyclic graph 
-    lemmaRemoveVertex(v, G');
-
     // remove that vertex and its outgoing edges from the graph
-    G' := removeVertex(v, G');
+    R := removeVertex(v, R);
   }
 }
 
+/** SECOND LEMMA ***/
 
-/** FIRST LEMMA ***/
-
-// States and proves the following property: a non-empty acyclic graph must have 
-// at least one vertex without incoming edges (0 indegree).  
-lemma lemmaAcyclic<T>(G: Graph<T>) 
+// States and proves by contradiction the following property: a non-empty acyclic graph 
+// must have at least one vertex without incoming edges (0 indegree).  
+lemma lemmaAcyclicIndegrees<T>(G: Graph<T>) 
   requires validGraph(G) && G.V != {} && acyclic(G)
-  ensures exists v :: v in G.V && !exists u :: u in G.V && (u, v) in G.E
+  ensures exists v :: v in G.V && !hasIncomingEdges(G, v)
 {
-  // Do the proof by contradiction. 
-  // Start by assuming that all vertices have incoming edges.
-  if forall v :: v in G.V ==> exists u :: u in G.V && (u, v) in G.E {
+  // For the sake of contradiction, assume that all vertices have incoming edges.
+  if forall v :: v in G.V ==> hasIncomingEdges(G, v) {
     // Then a path of any length can be built, possibly with repeated edges
     // and vertices, namely a path with length |G.V| + 1 
-    var p := genComplexPath(G, |G.V| + 1);
+    var p := genPath(G, |G.V| + 1);
     // Such a path must have repeated vertices, and consequently at least one cycle
-    lemmaComplexPathLen(G, p);
+    lemmaPathLen(G, p);
     // So the graph is not acyclic, which contradicts the pre-condition
     assert ! acyclic(G);
   }
@@ -105,40 +108,40 @@ lemma lemmaAcyclic<T>(G: Graph<T>)
 // in which all vertices have incoming edges.
 // Because of this property, a path with any length may be constructed (possibly
 // with repeated edges and vertices). 
-lemma genComplexPath<T> (G: Graph<T>, n: nat) returns (p: seq<T>)
+lemma genPath<T> (G: Graph<T>, n: nat) returns (p: seq<T>)
   requires validGraph(G) && G.V != {}  
-  requires forall v :: v in G.V ==> exists u :: u in G.V && (u, v) in G.E
-  ensures validComplexPath(p, G) && |p| == n
+  requires forall v :: v in G.V ==> hasIncomingEdges(G, v)
+  ensures |p| == n && validPath(p, G)
 {
   p := [];
   while |p| < n
-    invariant 0 <= |p| <= n && validComplexPath(p, G)
+    invariant |p| <= n && validPath(p, G)
   {
     var u :| u in G.V && (p == [] || (u, p[0]) in G.E);
     p := [u] + p;
   }
 }
 
-// Checks if a sequence p of vertices defines a valid complex path
+// Checks if a sequence p of vertices defines a valid  path
 // (allowing repeated vertices and edges) in a graph G.
-predicate method validComplexPath<T>(p: seq<T>, G: Graph<T>) {
+predicate method validPath<T>(p: seq<T>, G: Graph<T>) {
    forall i :: 0 <= i < |p| ==> p[i] in G.V
          && (i < |p| - 1 ==> (p[i], p[i+1]) in G.E)
 }
 
-// States and proves the property: given a non-empty graph G and a complex path p in G, 
+// States and proves the property: given a graph G and a path p in G, 
 // if the length of p exceeds the number of vertices then G has cycles.  
-lemma lemmaComplexPathLen<T>(G: Graph<T>, p: seq<T>)
-  requires validGraph(G) && G.V != {} && validComplexPath(p, G) && |p| > |G.V| 
+lemma lemmaPathLen<T>(G: Graph<T>, p: seq<T>)
+  requires validGraph(G) && validPath(p, G) && |p| > |G.V| 
   ensures !acyclic(G)
 {
   // first notice that, if all vertices are distinct, the length of the path 
   // cannot exceed the number of vertices in G 
-  if forall i, j :: 0 <= i < j < |p| ==> p[i] != p[j] {
+  if nodups(p) {
     lemmaSeqLen(p, G.V);
   }
 
-  // consequently, there must exist repeated vertice in p, so we pick
+  // consequently, there must exist repeated vertices in p, so we pick
   // a cyclic (complex) subpath 
   var i, j :| 0 <= i < j < |p| && p[i] == p[j];
   var p' := p[i .. j+1];
@@ -151,12 +154,12 @@ lemma lemmaComplexPathLen<T>(G: Graph<T>, p: seq<T>)
 // repeated edges and/or vertices) in a graph G, there exists a simple
 // path (without repeated edges) in G from the first to the last vertex in the complex path. 
 lemma lemmaComplexPath<T>(G: Graph<T>, p: seq<T>)
-  requires G.V != {} && validComplexPath(p, G) && |p| > 1
+  requires G.V != {} && validPath(p, G) && |p| > 1
   ensures existsSimplePath(G, p[0], p[|p|-1])
   decreases p
 {
-  // handles case of first edge repeated
-  if i :| 1 <= i < |p|-1 && p[i] == p[0] && p[i+1] == p[1] {
+  // handles case of first vertex repeated in the middle
+  if i :| 1 <= i < |p|-1 && p[i] == p[0] {
     lemmaComplexPath(G, p[i..]);
   }
   // handles recursive case of proof by induction
@@ -184,19 +187,18 @@ lemma lemmaSeqLen<T>(p: seq<T>, s: set<T>)
   }
 }
 
-/** SECOND LEMMA ***/
+/** FIRST LEMMA ***/
 
-// States and proves (by contradiction) the following property: removing a vertex 
-// v from an acyclic graph G produces an acyclic graph. 
-lemma lemmaRemoveVertex<T>(v: T, G: Graph<T>) 
-  requires validGraph(G) && acyclic(G) && v in G.V 
-  ensures acyclic(removeVertex(v, G))
+// States and proves (by contradiction) the following property: a subgraph G of
+// an acyclic graph G' is also acyclic.
+lemma lemmaAcyclicSubgraph<T>(G: Graph<T>, G': Graph<T>) 
+  requires validGraph(G) && validGraph(G') && acyclic(G') && isSubGraph(G, G')  
+  ensures acyclic(G)
 {
-  var G' := removeVertex(v, G);
-  if ! acyclic(G') {
-     var u :| u in G'.V && existsSimplePath(G', u, u); // exists, by the definition of acyclic
-     lemmaExistsSimplePath(G', G, u, u); // recall lemma implying that such a path also exists in G
-     assert !acyclic(G); // so, G would not be acyclic, contradicting the precondition
+  if ! acyclic(G) {
+     var u :| u in G.V && existsSimplePath(G, u, u); // exists, by the definition of acyclic
+     lemmaExistsSimplePath(G, G', u, u); // recall lemma implying that such a path also exists in G
+     assert !acyclic(G'); // so, G would not be acyclic, contradicting the precondition
   }
 }
 
@@ -205,10 +207,10 @@ predicate isSubGraph<T>(G: Graph<T>, G': Graph<T>) {
   G.E <= G'.E && G.V <= G'.V
 }
 
-// States and proves (by induction) the following property: if there is a (simple) path u-->v in a graph G
-// and G is a subgraph of G', then a path u-->v also exists in G'.
+// States and proves (by induction) the following property: if there is a (simple) path u-->v
+// in a graph G and G is a subgraph of G', then a path u-->v also exists in G'.
 lemma lemmaExistsSimplePath<T>(G: Graph<T>, G': Graph<T>, u: T, v: T)
-  requires validGraph(G) && validGraph(G') && isSubGraph(G, G') && u in G.V && v in G.V && existsSimplePath(G, u, v) 
+  requires validGraph(G) && validGraph(G') && isSubGraph(G, G') && existsSimplePath(G, u, v) 
   ensures existsSimplePath(G', u, v)
   decreases G.E
 { 
@@ -217,7 +219,6 @@ lemma lemmaExistsSimplePath<T>(G: Graph<T>, G': Graph<T>, u: T, v: T)
     lemmaExistsSimplePath(Graph(G.V, G.E-{e}), Graph(G'.V, G'.E-{e}), e.1, v); // this lemma implies that 'e' also exist in G' 
   } 
 }
-
 
 /** Test cases ***/
 method testTopSortingSingleSolution() {
@@ -239,4 +240,3 @@ method testTopSortingMultipleSolutions() {
   var t := topsort(G);
   assert t == s1 || t == s2;
 }
-
